Added example optimizations: canonical form of some AddNode and SubNode expressions.

GraalExprs.thy
@@ -2,7 +2,12 @@ theory GraalExprs
 imports Main
 begin
 
-type_synonym Stamp = int  (* TODO: build a representation of types *)
+(* Stamps are a kind of type system, with a lattice structure. *)
+datatype Stamp =
+  IntegerStamp |
+  FloatStamp
+  (* TODO: add other kinds of types *)
+
 
 section expressions
 (*========================================================================
@@ -25,7 +30,8 @@ we define those as predicates, named 'isa_<AbstractClassName>(n)'.
 *)
 
 datatype IRNode =
-  ConstantNode (*String? value*) int
+  NullNode  (* Not a real node, but used for some return values *)
+  | ConstantNode (*String? value*) int
   | ParameterNode (*index*) int
   | AddNode (*x*) IRNode (*y*) IRNode
   | SubNode (*x*) IRNode (*y*) IRNode
@@ -48,21 +54,29 @@ fun inputEdges :: "IRNode \<Rightarrow> IRNode list" where
   "inputEdges (ConstantNode i) = []" |
   "inputEdges (ParameterNode i) = []" |
   "inputEdges (AddNode x y) = [x, y]" |
-  "inputEdges (SubNode x y) = [x, y]"
+  "inputEdges (SubNode x y) = [x, y]" |
+  "inputEdges Null = []"
 
+
+(* isAssociative method (only for int expressions at the moment). *)
+fun isAssociative :: "IRNode \<Rightarrow> bool" where
+  "isAssociative (AddNode x y) = True" |
+  "isAssociative (SubNode x y) = True" |
+  "isAssociative _ = False"
 
 
 (* An example expression: (aa + 1) - aa *)
 abbreviation eg_aa :: IRNode where
   "eg_aa \<equiv> (ParameterNode 5)"
 
-(* Example of value equivalence of expressions. *)
+(* An example of value equivalence of expressions. *)
 lemma aa1_eq: "(AddNode eg_aa (ConstantNode 2)) = (AddNode eg_aa (ConstantNode (1+1)))"
   apply(simp)
   done
 
+(* (1 - aa) + aa *)
 abbreviation eg_a1a :: IRNode where
-  "eg_a1a \<equiv> (SubNode (AddNode eg_aa (ConstantNode 1)) eg_aa)"
+  "eg_a1a \<equiv> (AddNode (SubNode (ConstantNode 1) eg_aa) eg_aa)"
 
 lemma expr_a1a_binary [simp]: "isa_BinaryArithmeticNode(eg_a1a)"
   apply(simp add: isa_BinaryArithmeticNode_def)
@@ -76,11 +90,124 @@ lemma const_is_constant [simp]: "isConstant(ConstantNode i)"
 
 section canonical
 (*========================================================================
-This section is a translation of the 'AddNode/SubNode.canonical' optimization.
+This section is a translation of the 'AddNode/SubNode.canonical' optimizations.
 
 An example goal is to prove that canonical("(aa + 1) - aa)") returns "1".
 ========================================================================== *)
 
+(* These are partial translations of several Graal expression-optimization methods:
+   Limitations: we ignore stamps and views for now, and assume int expressions.
+*)
+
+(* From class BinaryArithmeticNode:
+    public static <OP> ConstantNode tryConstantFold(BinaryOp<OP> op, ValueNode forX, ValueNode forY, Stamp stamp, NodeView view) {
+        if (forX.isConstant() && forY.isConstant()) {
+            Constant ret = op.foldConstant(forX.asConstant(), forY.asConstant());
+            if (ret != null) {
+                return ConstantNode.forPrimitive(stamp, ret);
+            }
+        }
+        return null;
+    }
+*)
+
+(* Add only.  TODO: take Op (Add/Sub/Mul as a parameter *)
+fun BinArithTryConstFold :: "IRNode \<Rightarrow> IRNode \<Rightarrow> Stamp \<Rightarrow> IRNode" where
+  "BinArithTryConstFold (ConstantNode a) (ConstantNode b) stamp = ConstantNode (a+b)" |
+  "BinArithTryConstFold forX forY stamp = NullNode"
+
+
+(* From class AddNode:
+    private static ValueNode canonical(AddNode addNode, BinaryOp<Add> op, ValueNode forX, ValueNode forY, NodeView view) {
+        AddNode self = addNode;
+        boolean associative = op.isAssociative();
+        if (associative) {
+            if (forX instanceof SubNode) {
+                SubNode sub = (SubNode) forX;
+                if (sub.getY() == forY) {
+                    // (a - b) + b
+                    return sub.getX();
+                }
+            }
+            if (forY instanceof SubNode) {
+                SubNode sub = (SubNode) forY;
+                if (sub.getY() == forX) {
+                    // b + (a - b)
+                    return sub.getX();
+                }
+            }
+        }
+    // TODO:
+        if (forY.isConstant()) {
+            Constant c = forY.asConstant();
+            if (op.isNeutral(c)) {
+                return forX;
+            }
+            if (associative && self != null) {
+                // canonicalize expressions like "(a + 1) + 2"
+                ValueNode reassociated = reassociate(self, ValueNode.isConstantPredicate(), forX, forY, view);
+                if (reassociated != self) {
+                    return reassociated;
+                }
+            }
+            /* ignore optimisation of extend nodes between two adds ... */
+            }
+        }
+        if (forX instanceof NegateNode) {
+            return BinaryArithmeticNode.sub(forY, ((NegateNode) forX).getValue(), view);
+        } else if (forY instanceof NegateNode) {
+            return BinaryArithmeticNode.sub(forX, ((NegateNode) forY).getValue(), view);
+        }
+        if (self == null) {
+            self = (AddNode) new AddNode(forX, forY).maybeCommuteInputs();
+        }
+        return self;
+    }
+*)
+
+(* TODO: only apply first two rules if op is associative. *)
+
+(* PROBLEM: proving the function side-conditions. *)
+function AddNodeCanonical :: "IRNode \<Rightarrow> IRNode" where
+  "AddNodeCanonical (AddNode (SubNode a b) b) = a" |   (*  (a - b) + b  *)
+  "AddNodeCanonical (AddNode b (SubNode a b)) = a" |   (*  b + (a - b)  *)
+  "AddNodeCanonical (AddNode a b) = (AddNode a b)"
+    if "a \<noteq> (SubNode _ b) \<and> b \<noteq> (SubNode _ a)" 
+  apply(auto)
+
+
+(* From class AddNode:
+    public static ValueNode create(ValueNode x, ValueNode y, NodeView view) {
+        BinaryOp<Add> op = ArithmeticOpTable.forStamp(x.stamp(view)).getAdd();
+        Stamp stamp = op.foldStamp(x.stamp(view), y.stamp(view));
+        ConstantNode tryConstantFold = tryConstantFold(op, x, y, stamp, view);
+        if (tryConstantFold != null) {
+            return tryConstantFold;
+        }
+        if (x.isConstant() && !y.isConstant()) {
+            return canonical(null, op, y, x, view);
+        } else {
+            return canonical(null, op, x, y, view);
+        }
+    }
+*)
+
+
+function AddNodeCreate :: "IRNode \<Rightarrow> IRNode \<Rightarrow> IRNode" where
+  "AddNodeCreate x y = BinArithTryConstFold x y IntegerStamp"
+if "BinArithTryConstFold x y IntegerStamp \<noteq> NullNode" |
+  "AddNodeCreate x y = AddNodeCanonical y x"
+if "BinArithTryConstFold x y IntegerStamp = NullNode \<and> isConstant x \<and> \<not> isConstant y" |
+  "AddNodeCreate x y = AddNodeCanonical x y"
+if "BinArithTryConstFold x y IntegerStamp = NullNode \<and> (\<not> isConstant x \<or> isConstant y)"
+  apply(auto)
+  by fastforce
+
+
+
+(*  An example optimization.  *)
+theorem canon_a1a: "AddNodeCanonical eg_a1a = (ConstantNode 1)"
+  apply(simp)
 
 
 end
